clean up

Lean/Geo/Triangle/EncodingNew.lean
@@ -2,140 +2,11 @@ import Mathlib.Data.Fin.Basic
 import Mathlib.Data.List.Range
 import Geo.SAT.ToLeanSAT.EncodeProof
 import Geo.NGon.Var
+import Geo.NGon.EncodingNew
 
 namespace Geo
 
 open LeanSAT Var
-
-/-
-
-Overall, we have three sets of variables:
-
-∀ 1 ≤ a < b < c ≤ n:
-
-  s{a, b, c}       === signotope of points a b c
-  I{x, a, b, c}    === x is "Inside" triangle a b c
-  H{a, b, c}       === triangle a b c is a hole (i.e. no other points strictly inside)
-
-  Notably, while the I variables can be defined for any four distinct {x, a, b, c},
-  they only really matter when
-
-      a < b < c (which we may assume generally throughout)
-      a < x < c
-
-  because otherwise, x cannot be inside the triangle anyway, and so its variable
-  would automatically be set to false (via logic, not by the SAT solver).
-
-The contraints are:
-
-  ∀ 1 ≤ a < b < c ≤ n:
-
-  Orientation constraints:
-    ∀ {d}, c < d:
-      !s{a, b, c} ∨ !s{a, c, d} ∨  s{a, b, d} ≃  (s{a, b, c} ∧ s{a, c, d}) → s{a, b, d}
-      !s{a, b, c} ∨ !s{b, c d}  ∨  s{a, c, d} ≃  (s{a, b, c} ∧ s{b, c, d}) → s{a, c, d}
-
-      (We take the top grouping and do them again, except negating the actual variables)
-
-       s{a, b, c} ∨  s{a, c, d} ∨ !s{a, b, d} ≃  (!s{a, b, c} ∧ !s{a, c, d}) → !s{a, b, d}
-       s{a, b, c} ∨  s{b, c, d} ∨ !s{a, c, d} ≃  (!s{a, b, c} ∧ !s{b, c, d}) → !s{a, c, d}
-
-
-  The "inside triangles" constraints:
-
-    (We split on whether the candidate point "x" to be inside is before or after "b")
-    (Note(WN): the new pt_in_triangle doesn't need a split, can we backport that to encoding?)
-
-    ∀ {x}, a < x < b:
-      I{x, a, b, c} ↔ ((s{a, b, c} ↔ s{a, x, c}) ∧ (!s{a, x, b} ↔ s{a, b, c}))
-
-    ∀ {x}, b < x < c:
-      I{x, a, b, c} ↔ ((s{a, b, c} ↔ s{a, x, c}) ∧ (!s{b, x, c} ↔ s{a, b, c}))
-
-    (Notably, the only difference is the third "s" variable, noting which two triangle points "x" lies between.)
-
-    The way the constraints work is as follows:
-      - The first pair places "x" and "b" on the same side of the line segment "ac"
-      - The second pair places "x" below the line segment coming from "a" to "b", or going from "b" to "c"
-
-    In addition to "x" being between "a" and "c", this places "x" to be inside the triangle.
-
-  The "hole" constraints:
-
-    ∀ {x}, a < x < c, with x ≠ b:
-      I{x, a, b, c} → !H{a, b, c}           (If "x" is inside triangle abc, then triangle abc isn't a hole)
-
-  Finally, the UNSAT constraints to look for non-holes:
-    !H{a, b, c}                             (To satisfy the formula, every triangle cannot be a hole, i.e. it contains a point.)
-
-
-
-  The proof skeleton looks like:
-    ∃ {pts : Finset Point}, NoHoles pts → ∃ {τ : Assignment}, F(τ) = SAT
-
-  The contrapositive then gives us
-    ∀ {τ : Assignment}, F(τ) = UNSAT → ∀ {pts : Finset Point}, ∃ a hole.
--/
-
-
-def signotopeClause (a b c d : Fin n) : PropForm (Var n) :=
-  .all #[
-    -- (s{a, b, c} ∧ s{a, c, d}) → s{a, b, d}
-    .imp (.and (sigma a b c) (sigma a c d)) (sigma a b d)
-  , -- (s{a, b, c} ∧ s{b, c, d}) → s{a, c, d}
-    .imp (.and (sigma a b c) (sigma b c d)) (sigma a c d)
-  , -- (!s{a, b, c} ∧ !s{a, c, d}) → !s{a, b, d}
-    .imp (.and (.not (sigma a b c)) (.not (sigma a c d))) (.not (sigma a b d))
-  , -- (!s{a, b, c} ∧ !s{b, c, d}) → !s{a, c, d}
-    .imp (.and (.not (sigma a b c)) (.not (sigma b c d))) (.not (sigma a c d))
-  ]
-
-def signotopeClauses (n : Nat) : PropForm (Var n) :=
-  -- for all `a`, `b`, `c` with `a < b < c`
-  .forAll (Fin n) fun a =>
-  .forAll (Fin n) fun b =>
-  .guard (a < b) fun _ =>
-  .forAll (Fin n) fun c =>
-  .guard (b < c) fun _ =>
-  .forAll (Fin n) fun d =>
-  .guard (c < d) fun _ =>
-  signotopeClause a b c d
-
-def xIsInsideClause (a b c x : Fin n) : PropForm (Var n) :=
-  .all #[
-    -- a < x < b
-    .guard (a < x ∧ x < b) fun _ =>
-      -- NOTE(Bernardo): Each of those should be expressible as 8 clauses or so
-      -- I{x, a, b, c} ↔ ((s{a, b, c} ↔ s{a, x, c}) ∧ (!s{a, x, b} ↔ s{a, b, c}))
-      .iff (inside x a b c) (
-        .and (.iff (sigma a b c) (sigma a x c)) (.iff (.not (sigma a x b)) (sigma a b c)))
-  , -- b < x < c
-    .guard (b < x ∧ x < c) fun _ =>
-      -- I{x, a, b, c} ↔ ((s{a, b, c} ↔ s{a, x, c}) ∧ (!s{b, x, c} ↔ s{a, b, c}))
-      .iff (inside x a b c) (
-        .and (.iff (sigma a b c) (sigma a x c)) (.iff (.not (sigma b x c)) (sigma a b c)))
-  ]
-
-def insideClauses (n : Nat) : PropForm (Var n) :=
-  -- for all `a`, `b`, `c` with `a < b < c`
-  .forAll (Fin n) fun a =>
-  .forAll (Fin n) fun b =>
-  .guard (a < b) fun _ =>
-  .forAll (Fin n) fun c =>
-  .guard (b < c) fun _ =>
-  .forAll (Fin n) fun x =>
-  xIsInsideClause a b c x
-
-def holeDefClauses (n : Nat) : PropForm (Var n) :=
-  .forAll (Fin n) fun a =>
-  .forAll (Fin n) fun b =>
-  .guard (a < b) fun _ =>
-  .forAll (Fin n) fun c =>
-  .guard (b < c) fun _ =>
-  .iff (Var.hole a b c) <|
-    .forAll (Fin n) fun x =>
-    .guard (a < x ∧ x < c ∧ x ≠ b) fun _ =>
-    .not (Var.inside x a b c)
 
 def noHoleClauses (n : Nat) : PropForm (Var n) :=
   .forAll (Fin n) fun a =>
@@ -145,20 +16,11 @@ def noHoleClauses (n : Nat) : PropForm (Var n) :=
   .guard (b < c) fun _ =>
     .not (hole a b c)
 
-def leftmostCCWClauses (n : Nat) : PropForm (Var n) :=
-  .forAll (Fin n) fun a =>
-  .guard (⟨0, Fin.size_positive a⟩ < a) fun _ =>
-  .forAll (Fin n) fun b =>
-  .guard (a < b) fun _ =>
-    Var.sigma ⟨0, Fin.size_positive a⟩ a b
-
-def theEncoding (n : Nat) : PropForm (Var n) :=
-  .all #[
-    signotopeClauses n, insideClauses n, holeDefClauses n, noHoleClauses n, leftmostCCWClauses n
-  ]
+def triangleEncoding (n : Nat) : PropForm (Var n) :=
+  .and (baseEncoding n) (noHoleClauses n)
 
 open Model PropFun
-axiom cnfUnsat : ¬∃ τ : IVar → Prop, (Geo.theEncoding 10 |>.toICnf compare).2.eval τ
+axiom triangleCnfUnsat : ¬∃ τ : IVar → Prop, (Geo.triangleEncoding 10 |>.toICnf compare).2.eval τ
 
 -- set_option profiler true in
--- #eval let cnf := Geo.theEncoding 10 |>.toICnf compare; (cnf.size, cnf.maxVar)
+-- #eval let cnf := (Geo.triangleEncoding 10 |>.toICnf compare).2; (cnf.size, cnf.maxVar)
