Lean/Geo/Triangle/WBAssnNew.lean
@@ -4,6 +4,7 @@ import Geo.Definitions.Structures
 import Geo.Definitions.OrientationProperties
 import Geo.Orientations
 import Geo.Triangle.EncodingNew
+import Geo.NGon.WBAssnNew
 
 namespace Geo.WBPoints
 open List
@@ -13,141 +14,14 @@ open LeanSAT.Model PropFun
 
 open Point
 
-@[simp] def toPropAssn (w : WBPoints) : Var w.length → Prop
-  | .sigma a b c ..    => σ w[a] w[b] w[c] = .CCW
-  | .inside x a b c .. => σPtInTriangle w[x] w[a] w[b] w[c]
-  | .hole a b c ..     => σIsEmptyTriangleFor w[a] w[b] w[c] w.toFinset
-
-attribute [-simp] getElem_fin
-
-theorem satisfies_signotopeClause (w : WBPoints) (i j k l : Fin w.length) :
-    i < j → j < k → k < l → (signotopeClause i j k l).eval w.toPropAssn := by
-  simp [signotopeClause]
-  intro hij hjk hkl
-  have : [w[i], w[j], w[k], w[l]] <+ w.points := by
-    have : [w[i], w[j], w[k], w[l]] = [i,j,k,l].map w.points.get := by
-      simp [GetElem.getElem, List.getElem_eq_get]
-    rw [this]
-    apply map_get_sublist
-    have := hjk.trans hkl
-    simp [hij, hjk, hkl, hij.trans hjk, hij.trans this, this]
-  have s : Sorted₄ w[i] w[j] w[k] w[l] := w.sorted.to₄ this
-  have gp : InGeneralPosition₄ w[i] w[j] w[k] w[l] :=
-    PointListInGeneralPosition.to₄ w.gp this
-  constructor
-  . exact σ_prop₂ s gp
-  constructor
-  . exact σ_prop₁ s gp
-  constructor
-  . simp_rw [gp.gp₁.σ_iff, gp.gp₂.σ_iff, gp.gp₃.σ_iff]
-    exact σ_prop₄ s gp
-  . simp_rw [gp.gp₁.σ_iff, gp.gp₄.σ_iff, gp.gp₃.σ_iff]
-    exact σ_prop₃ s gp
-
-theorem satisfies_signotopeClauses (w : WBPoints) : (signotopeClauses w.length).eval w.toPropAssn := by
-  simp (config := {contextual := true}) [signotopeClauses, satisfies_signotopeClause]
-
-theorem insideDefs_aux₁ {a x b c : Point} : Sorted₄ a x b c → InGeneralPosition₄ a x b c →
-    (σPtInTriangle x a b c ↔
-      ((σ a b c = .CCW ↔ σ a x c = .CCW) ∧ (σ a x b ≠ .CCW ↔ σ a b c = .CCW))) := by
-  intro sorted gp
-  simp only [σPtInTriangle,
-    σ_perm₂ a b x,
-    σ_perm₂ a c x,
-    σ_perm₂ a c b,
-    σ_perm₂ b c x, σ_perm₁ b x c,
-    σ_perm₂ b c a, σ_perm₁ b a c,
-    gp.gp₁.σ_iff]
-  cases gp.gp₁.σ_cases <;> cases gp.gp₂.σ_cases <;> cases gp.gp₃.σ_cases <;>
-    cases gp.gp₄.σ_cases <;> simp_all
-  next h₁ h₂ h₃ h₄ =>
-    rw [σ_prop₁ sorted gp h₁ h₄] at h₃
-    contradiction
-  next h₁ h₂ h₃ h₄ =>
-    rw [σ_prop₃ sorted gp h₁ h₄] at h₃
-    contradiction
-
-theorem insideDefs_aux₂ {a b x c : Point} : Sorted₄ a b x c → InGeneralPosition₄ a b x c →
-    (σPtInTriangle x a b c ↔
-      ((σ a b c = .CCW ↔ σ a x c = .CCW) ∧ (σ b x c ≠ .CCW ↔ σ a b c = .CCW))) := by
-  intro sorted gp
-  simp only [σPtInTriangle,
-    σ_perm₂ a c x,
-    σ_perm₂ a c b,
-    σ_perm₂ b c x,
-    σ_perm₂ b c a, σ_perm₁ b a c,
-    gp.gp₄.σ_iff]
-  cases gp.gp₁.σ_cases <;> cases gp.gp₂.σ_cases <;> cases gp.gp₃.σ_cases <;> cases gp.gp₄.σ_cases <;> simp_all
-  next h₁ h₂ h₃ h₄ =>
-    rw [σ_prop₁ sorted gp h₁ h₄] at h₃
-    contradiction
-  next h₁ h₂ h₃ h₄ =>
-    rw [σ_prop₃ sorted gp h₁ h₄] at h₃
-    contradiction
-
-theorem satisfies_insideClauses (w : WBPoints) : (insideClauses w.length).eval w.toPropAssn := by
-  simp [insideClauses, xIsInsideClause]
-  intro a b hab c hbc x
-  constructor
-  · intro hax hxb
-    have : [w[a], w[x], w[b], w[c]] <+ w.points := by
-      have : [w[a], w[x], w[b], w[c]] = [a,x,b,c].map w.points.get := by
-        simp [GetElem.getElem, List.getElem_eq_get]
-      rw [this]
-      apply map_get_sublist
-      have : a < c := hab.trans hbc
-      have : x < c := hxb.trans hbc
-      simp [*]
-    exact insideDefs_aux₁ (w.sorted.to₄ this) (PointListInGeneralPosition.to₄ w.gp this)
-  · intro hbx hxc
-    have : [w[a], w[b], w[x], w[c]] <+ w.points := by
-      have : [w[a], w[b], w[x], w[c]] = [a,b,x,c].map w.points.get := by
-        simp [GetElem.getElem, List.getElem_eq_get]
-      rw [this]
-      apply map_get_sublist
-      have : a < x := hab.trans hbx
-      have : a < c := hab.trans hbc
-      simp [*]
-    exact insideDefs_aux₂ (w.sorted.to₄ this) (PointListInGeneralPosition.to₄ w.gp this)
-
-theorem satisfies_holeDefClauses (w : WBPoints) : (holeDefClauses w.length).eval w.toPropAssn := by
-  simp [holeDefClauses, σIsEmptyTriangleFor, mem_toFinset_iff]
-  intro a b ab c bc
-  refine ⟨fun H _ _ _ _ => H _, fun H i tri => ?_⟩
-  have sub : [w[a],w[b],w[c]] <+ w.points := by
-    have : [w[a],w[b],w[c]] = [a,b,c].map w.points.get := by
-      simp [GetElem.getElem, List.getElem_eq_get]
-    rw [this]
-    apply map_get_sublist
-    aesop (add unsafe lt_trans)
-  have gp₄ : InGeneralPosition₄ w[i] w[a] w[b] w[c] := tri.gp₄_of_gp₃ (w.gp sub)
-  have ib : i ≠ b := mt (congrArg (w[·])) gp₄.gp₃.ne₁
-  have ⟨wawi, wiwc⟩ := xBounded_of_PtInTriangle (w.sorted.to₃ sub) ((σPtInTriangle_iff gp₄).mp tri)
-  have ai : a < i := w.of_sorted_get <| by
-    apply lt_of_le_of_ne wawi
-    intro h
-    exact gp₄.gp₁.ne₁ <| w.of_eqx h.symm ▸ rfl
-  have ic : i < c := w.of_sorted_get <| by
-    apply lt_of_le_of_ne wiwc
-    intro h
-    exact gp₄.gp₃.ne₂ <| w.of_eqx h ▸ rfl
-  exact H i ai ic ib tri
-
-theorem satisfies_leftmostCCWDefs (w : WBPoints) : (leftmostCCWClauses w.length).eval w.toPropAssn := by
-  simp [leftmostCCWClauses]
-  intro i h0i j hij
-  let ⟨i+1, hi⟩ := i; let ⟨j+1, hj⟩ := j
-  exact List.pairwise_iff_get.1 w.oriented
-    ⟨_, Nat.lt_of_succ_lt_succ hi⟩ ⟨_, Nat.lt_of_succ_lt_succ hj⟩ (Nat.lt_of_succ_lt_succ hij)
-
-theorem satisfies_noHoles (w : WBPoints) :
+theorem satisfies_triangleEncoding (w : WBPoints) :
     ¬σHasEmptyTriangle w.toFinset →
-    (theEncoding w.length).eval w.toPropAssn := by
-  simp [theEncoding, satisfies_signotopeClauses, satisfies_insideClauses, satisfies_holeDefClauses,
-    satisfies_leftmostCCWDefs, noHoleClauses, σIsEmptyTriangleFor, mem_toFinset_iff, σHasEmptyTriangle]
+    (triangleEncoding w.length).eval w.toPropAssn := by
+  simp [triangleEncoding, satisfies_baseEncoding, noHoleClauses,
+    σIsEmptyTriangleFor, mem_toFinset_iff, σHasEmptyTriangle]
   intro noholes a b hab c hbc
-  exact noholes a b (ne_of_lt hab <| w.of_eqx <| · ▸ rfl)
-                  c (ne_of_lt (hab.trans hbc) <| w.of_eqx <| · ▸ rfl)
-                    (ne_of_lt hbc <| w.of_eqx <| · ▸ rfl)
+  exact noholes a b (ne_of_lt hab <| w.eq_iff.1 <| · ▸ rfl)
+                  c (ne_of_lt (hab.trans hbc) <| w.eq_iff.1 <| · ▸ rfl)
+                    (ne_of_lt hbc <| w.eq_iff.1 <| · ▸ rfl)
 
 end WBPoints
