Lean/Geo/Hexagon/EncodingNew.lean
@@ -1,0 +1,107 @@
+import Mathlib.Data.Fin.Basic
+import Mathlib.Data.List.Range
+import Geo.SAT.ToLeanSAT.EncodeProof
+import Geo.NGon.Var
+import Geo.NGon.EncodingNew
+
+namespace Geo
+
+open LeanSAT Var
+
+-- cap a c d:    b  c
+--            a ------ d
+def capDef (a b c d : Fin n) : PropForm (Var n) :=
+  .imp (.and (.not (Var.sigma a b c)) (.not (Var.sigma b c d))) (Var.cap a c d)
+
+def capDef2 (a c d : Fin n) : PropForm (Var n) :=
+  .imp (Var.cap a c d) (.not (Var.sigma a c d))
+
+--            a ------ d
+-- cup a c d:    b  c
+def cupDef (a b c d : Fin n) : PropForm (Var n) :=
+  .imp (.and (Var.sigma a b c) (Var.sigma b c d)) (Var.cup a c d)
+
+def cupDef2 (a c d : Fin n) : PropForm (Var n) :=
+  .imp (Var.cup a c d) (Var.sigma a c d)
+
+--                .   b
+-- capF a c d:            c      (where a-b-d is a hole)
+--             a ---------- d
+def capFDef (a b c d : Fin n) : PropForm (Var n) :=
+  /- Var.hole a b d -> -/ .imp (.and (.not (Var.sigma b c d)) (Var.cap a b c)) (Var.capF a c d)
+
+-- a ----------- d
+--   ·         c
+--        b
+def no6Hole3Below (a b c d : Fin n) : PropForm (Var n) :=
+  /- Var.hole a b d -> -/ .imp (Var.cup a b c) (.not (Var.sigma b c d))
+
+--       .  b
+--   ·         c
+-- a ----------- d
+def no6Hole4Above (a b c d : Fin n) : PropForm (Var n) :=
+  .imp (Var.capF a b c) (Var.sigma b c d)
+
+def no6HoleClauses1 (n : Nat) : PropForm (Var n) :=
+  .forAll (Fin n) fun a =>
+  .guard (⟨0, Fin.size_positive a⟩ < a) fun _ =>
+  .forAll (Fin n) fun b =>
+  .guard (a < b) fun _ =>
+  .forAll (Fin n) fun c =>
+  .guard (b < c) fun _ =>
+  .forAll (Fin n) fun d =>
+  .guard (c < d) fun _ =>
+  .flatCNF <| .all #[
+    capDef a b c d, cupDef a b c d,
+    .guard (a.1+1 < b.1) fun _ => .all #[
+      .imp (Var.hole a b d) <| .all #[capFDef a b c d, no6Hole3Below a b c d],
+      .guard (a.1+2 < b.1) fun _ => no6Hole4Above a b c d
+    ]
+  ]
+
+def no6HoleClauses2 (n : Nat) : PropForm (Var n) :=
+  .forAll (Fin n) fun a =>
+  .guard (⟨0, Fin.size_positive a⟩ < a) fun _ =>
+  .forAll (Fin n) fun c =>
+  .guard (a.1+1 < c.1) fun _ =>
+  .forAll (Fin n) fun d =>
+  .guard (c < d) fun _ =>
+  .all #[capDef2 a c d, cupDef2 a c d]
+
+--     ·   p
+-- a --------- c
+--     ·   b
+def no6Hole2Below (a b c p : Fin n) : PropForm (Var n) :=
+  .not <| .all #[Var.cup a b c, Var.cap a p c,
+    if b < p then Var.hole a b p else Var.hole a p b]
+
+--        ·
+--   ·         b
+-- a ----------- c
+--         p
+def no6Hole1Below (a b c p : Fin n) : PropForm (Var n) :=
+  .imp (Var.capF a b c) <| .not (Var.sigma a p c)
+
+def no6HoleClauses3 (n : Nat) : PropForm (Var n) :=
+  .forAll (Fin n) fun a =>
+  .guard (⟨0, Fin.size_positive a⟩ < a) fun _ =>
+  .forAll (Fin n) fun b =>
+  .guard (a < b) fun _ =>
+  .forAll (Fin n) fun c =>
+  .guard (b < c) fun _ =>
+  .forAll (Fin n) fun p =>
+  .guard (a < p ∧ p < c ∧ b ≠ p) fun _ =>
+  .all #[
+    .guard (a.1 + 1 < b.1 ∧ a.1 + 1 < p.1) fun _ => no6Hole2Below a b c p,
+    .guard (a.1 + 2 < b.1) fun _ => no6Hole1Below a b c p
+  ]
+
+
+def hexagonEncoding (n : Nat) : PropForm (Var n) :=
+  .all #[baseEncoding n, no6HoleClauses1 n, no6HoleClauses2 n, no6HoleClauses3 n]
+
+open Model PropFun
+axiom hexagonCnfUnsat : ¬∃ τ : IVar → Prop, (Geo.hexagonEncoding 30 |>.toICnf compare).2.eval τ
+
+-- set_option profiler true in
+-- #eval let cnf := (Geo.triangleEncoding 10 |>.toICnf compare).2; (cnf.size, cnf.maxVar)
