Lean/Geo/Hexagon/TheMainTheoremNew.lean
@@ -1,0 +1,22 @@
+import Geo.PointsToWB.SymmetryBreakingNew
+import Geo.SigmaEquiv
+import Geo.Hexagon.WBAssnNew
+import Geo.Hexagon.EncodingNew
+
+namespace Geo
+open List Classical
+
+theorem EmptyHexagon30TheoremLists (pts : List Point) (gp : Point.PointListInGeneralPosition pts) (h : pts.length = 30) :
+    HasEmptyNGon 6 pts.toFinset := by
+  by_contra h'
+  have noσtri : ¬σHasEmptyNGon 6 pts.toFinset := mt (σHasEmptyNGon_iff_HasEmptyNGon gp).1 h'
+  have ⟨w, ⟨hw⟩⟩ := @symmetry_breaking pts (h ▸ by decide) gp
+  have noσtri' : ¬σHasEmptyNGon 6 w.toFinset :=
+    OrientationProperty_σHasEmptyNGon.not (hw.toEquiv w.nodup) noσtri
+  have len10 : w.length = 30 := hw.length_eq.symm.trans h
+  with_reducible have := (LeanSAT.PropForm.toICnf_sat _).2 ⟨w.toPropAssn, w.satisfies_hexagonEncoding noσtri'⟩
+  rw [len10] at this
+  exact hexagonCnfUnsat this
+
+/- 'Geo.EmptyHexagon10TheoremLists' depends on axioms: [propext, Classical.choice, Quot.sound, Geo.cnfUnsat] -/
+#print axioms EmptyHexagon30TheoremLists
