Lean/Geo/Triangle/TheMainTheoremNew.lean
@@ -8,87 +8,17 @@ namespace Geo
 open List
 open Classical
 
-lemma HasEmptyTriangle_iff_σHasEmptyTriangle (gp : Point.PointListInGeneralPosition pts) :
-    σHasEmptyTriangle pts.toFinset ↔ HasEmptyTriangle pts.toFinset := by
-  rw [HasEmptyTriangle.iff]
-  constructor
-  . intro ⟨a, ha, b, hb, c, hc, ab, ac, bc, empty⟩
-    use a, ha, b, hb, c, hc
-    have gp₃ : Point.InGeneralPosition₃ a b c := by
-      apply Point.PointListInGeneralPosition.subperm.mp gp
-      apply List.subperm_of_subset (by simp [*])
-      sublist_tac
-    refine ⟨gp₃, ?_⟩
-    intro s hs tri
-    simp only [coe_toFinset, Set.mem_diff, Set.mem_setOf_eq, Set.mem_insert_iff,
-      Set.mem_singleton_iff, not_or] at hs
-    have ⟨hs, _, _, _⟩ := hs
-    apply empty s (by simp [hs])
-    rwa [σPtInTriangle_iff]
-    apply gp.subperm₄
-    apply List.subperm_of_subset (by simp [*])
-    sublist_tac
-  . intro ⟨a, ha, b, hb, c, hc, gp', empty⟩
-    use a, ha, b, hb, c, hc, gp'.ne₁, gp'.ne₂, gp'.ne₃
-    intro s hs
-    by_cases sb : s = b
-    . rw [sb]
-      apply not_mem_σPtInTriangle gp'
-    by_cases sa : s = a
-    . intro h
-      apply not_mem_σPtInTriangle gp'.perm₁
-      apply σPtInTriangle.perm₁
-      rwa [sa] at h
-    by_cases sc : s = c
-    . intro h
-      apply not_mem_σPtInTriangle gp'.perm₂
-      apply σPtInTriangle.perm₂
-      rwa [sc] at h
-    have gp₄ : Point.InGeneralPosition₄ s a b c := by
-      apply gp.subperm₄
-      apply List.subperm_of_subset (by simp [*, gp'.ne₁, gp'.ne₂, gp'.ne₃])
-      sublist_tac
-    rw [σPtInTriangle_iff gp₄]
-    apply empty
-    simp at hs
-    simp [hs, not_or, *]
-
-lemma OrientationProperty_σHasEmptyTriangle : OrientationProperty σHasEmptyTriangle := by
-  unfold σHasEmptyTriangle
-  intro S T ST ⟨a, ha, b, hb, c, hc, ab, ac, bc, empty⟩
-  refine ⟨ST ⟨a, ha⟩, Subtype.property _, ST ⟨b, hb⟩, Subtype.property _, ST ⟨c, hc⟩, Subtype.property _, ?_⟩
-  simp [Subtype.coe_injective.eq_iff, ab, ac, bc]
-  intro s hs ⟨tri₁, tri₂, tri₃⟩
-  apply empty (ST.symm ⟨s, hs⟩) (Subtype.property _)
-  refine ⟨?_, ?_, ?_⟩
-  . have := ST.symm.hσ (ST ⟨a, ha⟩) (ST ⟨b, hb⟩) ⟨s, hs⟩
-    rw [this] at tri₁
-    have := ST.hσ ⟨a, ha⟩ ⟨b, hb⟩ ⟨c, hc⟩
-    have := tri₁.trans this.symm
-    simpa using this
-  . have := ST.symm.hσ (ST ⟨a, ha⟩) (ST ⟨c, hc⟩) ⟨s, hs⟩
-    rw [this] at tri₂
-    have := ST.hσ ⟨a, ha⟩ ⟨c, hc⟩ ⟨b, hb⟩
-    have := tri₂.trans this.symm
-    simpa using this
-  . have := ST.symm.hσ (ST ⟨b, hb⟩) (ST ⟨c, hc⟩) ⟨s, hs⟩
-    rw [this] at tri₃
-    have := ST.hσ ⟨b, hb⟩ ⟨c, hc⟩ ⟨a, ha⟩
-    have := tri₃.trans this.symm
-    simpa using this
-
-open LeanSAT.Model.PropFun in
 theorem EmptyTriangle10TheoremLists (pts : List Point) (gp : Point.PointListInGeneralPosition pts) (h : pts.length = 10) :
     HasEmptyTriangle pts.toFinset := by
   by_contra h'
-  have noσtri : ¬σHasEmptyTriangle pts.toFinset := mt (HasEmptyTriangle_iff_σHasEmptyTriangle gp).1 h'
+  have noσtri : ¬σHasEmptyTriangle pts.toFinset := mt (σHasEmptyTriangle_iff_HasEmptyTriangle gp).1 h'
   have ⟨w, ⟨hw⟩⟩ := @symmetry_breaking pts (h ▸ by decide) gp
   have noσtri' : ¬σHasEmptyTriangle w.toFinset :=
     OrientationProperty_σHasEmptyTriangle.not (hw.toEquiv w.nodup) noσtri
   have len10 : w.length = 10 := hw.length_eq.symm.trans h
-  with_reducible have := (LeanSAT.PropForm.toICnf_sat _).2 ⟨w.toPropAssn, w.satisfies_noHoles noσtri'⟩
+  with_reducible have := (LeanSAT.PropForm.toICnf_sat _).2 ⟨w.toPropAssn, w.satisfies_triangleEncoding noσtri'⟩
   rw [len10] at this
-  exact cnfUnsat this
+  exact triangleCnfUnsat this
 
 /- 'Geo.EmptyTriangle10TheoremLists' depends on axioms: [propext, Classical.choice, Quot.sound, Geo.cnfUnsat] -/
 #print axioms EmptyTriangle10TheoremLists
